theories/syntax/module.v
@@ -1,5 +1,9 @@
 Require Import RichWasm.syntax.rw.
 
+Record module_type :=
+  { mt_imports : list function_type;
+    mt_exports : list function_type }.
+
 Record module_function :=
   { mf_type : function_type;
     mf_locals : list representation;
