theories/iris/logrel/fundamental_module.v
@@ -1,0 +1,19 @@
+Require Import RichWasm.typing.
+Require Import RichWasm.compiler.module.
+Require Import RichWasm.iris.rules.iris_rules.
+Require Import RichWasm.iris.logrel.relations.
+
+Set Bullet Behavior "Strict Subproofs".
+Set Default Goal Selector "!".
+
+Section Fundamental.
+
+  Context `{Σ : gFunctors}.
+
+  Theorem fundamental_module m m' ω :
+    has_module_type m ω ->
+    run_modgen (compile_module m) mod_empty = inr (tt, m') ->
+    ⊢ @has_module_type_sem Σ m' ω.
+  Admitted.
+
+End Fundamental.
