theories/syntax.v
@@ -1,13 +1,23 @@
 From Stdlib Require Import List.
 Import ListNotations.
 
+Require Import RecordUpdate.RecordUpdate.
+
 From RichWasm.syntax Require Export module rw.
 
-Fixpoint flatten_func_type (ϕ : function_type) : list kind * list type * list type :=
+Record flat_function_type :=
+  { fft_mem_vars : nat;
+    fft_rep_vars : nat;
+    fft_size_vars : nat;
+    fft_type_vars : list kind;
+    fft_in : list type;
+    fft_out : list type }.
+
+Fixpoint flatten_function_type (ϕ : function_type) : flat_function_type :=
   match ϕ with
-  | MonoFunT τs1 τs2 => ([], τs1, τs2)
-  | ForallMemT ϕ'
-  | ForallRepT ϕ'
-  | ForallSizeT ϕ' => flatten_func_type ϕ'
-  | ForallTypeT κ ϕ' => let '(κs, τs1, τs2) := flatten_func_type ϕ' in (κ :: κs, τs1, τs2)
+  | MonoFunT τs1 τs2 => Build_flat_function_type 0 0 0 [] τs1 τs2
+  | ForallMemT ϕ' => flatten_function_type ϕ' <| fft_mem_vars ::= S |>
+  | ForallRepT ϕ' => flatten_function_type ϕ' <| fft_rep_vars ::= S |>
+  | ForallSizeT ϕ' => flatten_function_type ϕ' <| fft_size_vars ::= S |>
+  | ForallTypeT κ ϕ' => flatten_function_type ϕ' <| fft_type_vars ::= app [κ] |>
   end.
